Prove all theorems in computeSyntax

candle/prover/computeSyntaxScript.sml
@@ -32,9 +32,7 @@ Definition numeral_thy_ok_def:
     term_ok (sigof thy) _SUC ∧
     term_ok (sigof thy) _ADD ∧
     (* BIT0, BIT1 *)
-    (thy,[]) |- Comb _BIT0 _0 === _0 ∧
-    (thy,[]) |- Comb _BIT0 (Comb _SUC _N) ===
-                 Comb _SUC (Comb _SUC (Comb _BIT0 _N)) ∧
+    (thy,[]) |- Comb _BIT0 _N === Comb (Comb _ADD _N) _N ∧
     (thy,[]) |- Comb _BIT1 _N === Comb _SUC (Comb _BIT0 _N) ∧
     (* ADD *)
     (thy,[]) |- Comb (Comb _ADD _0) _M === _M ∧
@@ -73,28 +71,21 @@ Proof
   Induct_on ‘n’ \\ rw [numeral_thy_ok_def, term_ok_def, num2term_def]
 QED
 
+Theorem num2term_VSUBST[local,simp]:
+  ∀n. VSUBST is (num2term n) = num2term n
+Proof
+  Induct \\ rw [num2term_def, VSUBST_def]
+QED
+
 Definition num2bit_def:
-  num2bit n = if n = 0 then
-                Comb _BIT0 _0
-              else if n MOD 2 = 0 then
-                Comb _BIT0 (num2bit (n DIV 2))
-              else
-                Comb _BIT1 (num2bit (n DIV 2))
+  num2bit n =
+    if n = 0 then
+      Comb _BIT0 _0
+    else
+      Comb (if n MOD 2 = 0 then _BIT0 else _BIT1) (num2bit (n DIV 2))
 Termination
   wf_rel_tac ‘$<’ \\ intLib.ARITH_TAC
 End
-
-(*
-Theorem num2bit2:
-  ∀n.
-    (num2bit (2 * n) = Comb _BIT0 (if n = 0 then _0 else num2bit n)) ∧
-    (num2bit (SUC (2 * n)) = Comb _BIT1 (num2bit n))
-Proof
-  ho_match_mp_tac num2bit_ind \\ rw []
-  \\ rw [Once num2bit_def]
-  \\ gs [DIV_EQ_0, DECIDE “∀n. n < 2n ⇔ n = 0 ∨ n = 1”, ADD1]
-QED
- *)
 
 Theorem num2bit_typeof[local,simp]:
   ∀n. typeof (num2bit n) = num_ty
@@ -128,41 +119,57 @@ Proof
   \\ rw [Once num2bit_def, term_ok_def]
 QED
 
-Theorem replaceL1:
-  theory_ok thy ∧
-  term_ok (sigof thy) f ∧ welltyped f ∧
-  term_ok (sigof thy) x ∧ welltyped x ∧
-  term_ok (sigof thy) g ∧ welltyped g ∧
-  typeof f = Fun (typeof x) ty ∧
-  typeof g = Fun (typeof x) ty ∧
-  (thy,[]) |- f === g ∧
-  (thy,[]) |- Comb f x === z ⇒
-    (thy,[]) |- Comb g x === z
+Theorem num2bit_VSUBST[local,simp]:
+  ∀n. VSUBST is (num2bit n) = num2bit n
 Proof
-  strip_tac
-  \\ qspecl_then [‘t’,‘[]’,‘[]’] (irule o SIMPR []) trans_equation
-  \\ irule_at Any ACONV_REFL
-  \\ first_assum (irule_at Any)
-  \\ qspecl_then [‘[]’,‘[]’] (irule o SIMPR []) proves_MK_COMB
-  \\ simp [sym_equation, proves_REFL]
+  ho_match_mp_tac num2bit_ind \\ rw []
+  \\ once_rewrite_tac [num2bit_def]
+  \\ rw [VSUBST_def]
 QED
 
-Theorem replaceL2:
+Theorem trans_equation_simple[local]:
+  (thy,[]) |- a === b ∧
+  (thy,[]) |- b === c ⇒
+    (thy,[]) |- a === c
+Proof
+  rw []
+  \\ qspecl_then [‘t’,‘[]’,‘[]’] (irule o SIMPR []) trans_equation
+  \\ simp [ACONV_REFL, SF SFY_ss]
+QED
+
+Theorem MK_COMB_simple[local] =
+  Q.SPECL [‘[]’,‘[]’] proves_MK_COMB |> SIMPR [PULL_EXISTS];
+
+Theorem replaceL1[local]:
   theory_ok thy ∧
-  term_ok (sigof thy) f ∧ welltyped f ∧
-  term_ok (sigof thy) x ∧ welltyped x ∧
+  EVERY (term_ok (sigof thy)) [f; g; x] ∧
   typeof f = Fun (typeof x) ty ∧
-  typeof x = typeof y ∧ welltyped y ∧
+  typeof g = Fun (typeof x) ty ⇒
+    (thy,[]) |- f === g ∧
+    (thy,[]) |- Comb f x === z ⇒
+      (thy,[]) |- Comb g x === z
+Proof
+  rw []
+  \\ irule trans_equation_simple
+  \\ first_assum (irule_at Any)
+  \\ simp [MK_COMB_simple, term_ok_welltyped, proves_REFL, sym_equation,
+           SF SFY_ss]
+QED
+
+Theorem replaceL2[local]:
+  theory_ok thy ∧
+  EVERY (term_ok (sigof thy)) [f;x;y] ∧
+  typeof f = Fun (typeof x) ty ∧
+  typeof x = typeof y ∧
   (thy,[]) |- x === y ∧
   (thy,[]) |- Comb f x === z ⇒
     (thy,[]) |- Comb f y === z
 Proof
-  strip_tac
-  \\ qspecl_then [‘t’,‘[]’,‘[]’] (irule o SIMPR []) trans_equation
-  \\ irule_at Any ACONV_REFL
+  rw []
+  \\ irule trans_equation_simple
   \\ first_assum (irule_at Any)
-  \\ qspecl_then [‘[]’,‘[]’] (irule o SIMPR []) proves_MK_COMB
-  \\ simp [sym_equation, proves_REFL]
+  \\ simp [MK_COMB_simple, term_ok_welltyped, proves_REFL, sym_equation,
+           SF SFY_ss]
 QED
 
 Theorem replaceR1 =
@@ -171,143 +178,11 @@ Theorem replaceR1 =
 Theorem replaceR2 =
   UNDISCH_ALL replaceL2 |> MATCH_MP sym_equation |> DISCH_ALL;
 
-(*
-Theorem subst1:
-  theory_ok thy ∧
-  term_ok (sigof thy) x ∧ welltyped x ∧ x has_type ty ∧
-  typeof f' = typeof f ∧ typeof f = Fun ty rty ∧
-  VSUBST [x,Var n ty] f' = f ∧
-  VSUBST [x,Var n ty] g' = g ∧
-  (thy,[]) |- Comb f' (Var n ty) === Comb g' (Var n ty) ⇒
-    (thy,[]) |- Comb f x === Comb g x
-Proof
-  strip_tac
-  \\ drule_at_then (Pos (el 2)) (qspec_then ‘[x,Var n ty]’ mp_tac)
-                   proves_INST
-  \\ simp [VSUBST_def, equation_def, REV_ASSOCD]
-QED
- *)
-
-(*
-Theorem const_subst_idem[local]:
-  VSUBST is _BIT0 = _BIT0 ∧
-  VSUBST is _BIT1 = _BIT1 ∧
-  VSUBST is _SUC = _SUC ∧
-  VSUBST is _0 = _0
-Proof
-  rw [VSUBST_def]
-QED
-
-val [VSUBST_BIT0,VSUBST_BIT1,VSUBST_SUC,VSUBST_0] =
-  CONJUNCTS const_subst_idem;
- *)
-
-Theorem num2term_BIT0:
-  numeral_thy_ok thy ⇒
-    ∀n. (thy,[]) |- Comb _BIT0 (num2term (SUC n DIV 2)) === num2term n
-Proof
-  cheat
-QED
-
-Theorem num2bit_num2term:
-  numeral_thy_ok thy ⇒
-    ∀n. (thy,[]) |- num2bit n === num2term n
-Proof
-  strip_tac \\ ho_match_mp_tac num2bit_ind
-  \\ Cases \\ rw [num2term_def, Once num2bit_def]
-  \\ gs [numeral_thy_ok_def]
-  \\ rename [‘SUC n’]
-  \\ ‘∀n. typeof (num2bit n) = num_ty ∧
-          welltyped (num2bit n) ∧
-          num2bit n has_type num_ty ∧
-          term_ok (sigof thy) (num2bit n)’
-    by cheat (* TODO *)
-  \\ ‘∀n. typeof (num2term n) = num_ty ∧
-          welltyped (num2term n) ∧
-          num2term n has_type num_ty ∧
-          term_ok (sigof thy) (num2term n)’
-    by cheat (* TODO *)
-  \\ qabbrev_tac ‘N = Comb _BIT0 _0’
-  \\ ‘N has_type num_ty ∧ welltyped N’
-    by metis_tac [has_type_rules, welltyped_def]
-  \\ ‘typeof N = num_ty ∧ term_ok (sigof thy) N’
-    by simp [term_ok_def, typeof_def, Abbr ‘N’]
-  >- (
-    gvs [DIV_EQ_0, DECIDE “n < 2n ⇔ n = 0 ∨ n = 1”]
-    \\ rw [Once num2bit_def, num2term_def] \\ rw [Once num2bit_def]
-    \\ gs [Once num2bit_def]
-    \\ irule replaceR2 \\ gs []
-    \\ first_assum (irule_at Any) \\ simp []
-    \\ irule sym_equation
-    \\ qspecl_then [‘t’,‘[]’,‘[]’] (irule o SIMPR []) trans_equation
-    \\ irule_at Any ACONV_REFL
-    \\ ‘(thy,[]) |- Comb _BIT1 N === Comb _SUC (Comb _BIT0 N)’
-      by (qpat_x_assum ‘_ |- Comb _BIT1 _ === _’ assume_tac
-          \\ drule_at_then (Pos (el 2)) (qspec_then ‘[N,_N]’ mp_tac) proves_INST
-          \\ simp [VSUBST_def, REV_ASSOCD, equation_def, Abbr ‘N’, term_ok_def]
-          \\ disch_then irule
-          \\ simp [Abbr ‘N’, term_ok_def])
-    \\ pop_assum (irule_at Any)
-    \\ qspecl_then [‘[]’,‘[]’] (irule o SIMPR []) proves_MK_COMB
-    \\ simp [typeof_def, proves_REFL]
-    \\ ‘(thy,[]) |- Comb _BIT0 N === Comb _BIT0 _0’
-      by (qspecl_then [‘[]’,‘[]’] (irule o SIMPR []) proves_MK_COMB
-          \\ simp [typeof_def, proves_REFL])
-    \\ qspecl_then [‘t’,‘[]’,‘[]’] (irule o SIMPR []) trans_equation
-    \\ irule_at Any ACONV_REFL
-    \\ first_assum (irule_at Any)
-    \\ simp [proves_REFL])
-  >- (
-    cheat (*
-    Cases_on ‘SUC n MOD 2 = 0’ \\ gs []
-    >- (
-      rgs [Once MOD_EQ_0_DIVISOR] \\ gvs []
-      \\ simp [num2bit2]
-      \\ ‘(thy,[]) |- Comb _BIT0 (num2bit d) === Comb _BIT0 (num2term d)’
-        by (qspecl_then [‘[]’,‘[]’] (irule o SIMPR []) proves_MK_COMB
-            \\ simp [proves_REFL])
-      \\ qspecl_then [‘t’,‘[]’,‘[]’] (irule o SIMPR []) trans_equation
-      \\ irule_at Any ACONV_REFL
-      \\ first_assum (irule_at Any)
-      \\ ‘∃e. d = SUC e’ by intLib.ARITH_TAC \\ gvs []
-      \\ ‘n = SUC (2 * e)’ by intLib.ARITH_TAC \\ gvs []
-      \\ simp [num2term_def]
-      \\ cheat (* TODO bleh *))
-    \\ rgs [MOD_EQ_0_DIVISOR] \\ gvs []
-    \\ ‘SUC n = SUC (2 * (2 * d))’ by intLib.ARITH_TAC
-    \\ pop_assum SUBST1_TAC \\ simp [num2bit2]
-    \\ qabbrev_tac ‘M = Comb _BIT0 (num2bit d)’
-    \\ ‘M has_type num_ty ∧ term_ok (sigof thy) M’
-      by cheat (* TODO *)
-    \\ ‘(thy,[]) |- Comb _BIT1 M === Comb _SUC (Comb _BIT0 M)’
-      by (qpat_x_assum ‘_ |- Comb _BIT1 _ === _’ assume_tac
-          \\ drule_at_then (Pos (el 2)) (qspec_then ‘[M,_N]’ mp_tac) proves_INST
-          \\ simp [VSUBST_def, REV_ASSOCD, equation_def])
-    \\ qspecl_then [‘t’,‘[]’,‘[]’] (irule o SIMPR []) trans_equation
-    \\ irule_at Any ACONV_REFL
-    \\ first_assum (irule_at Any)
-    \\ qunabbrev_tac ‘M’
-    \\ qspecl_then [‘[]’,‘[]’] (irule o SIMPR []) proves_MK_COMB
-    \\ simp [proves_REFL]
-    \\ ‘(thy,[]) |- Comb _BIT0 (num2term (2 * d)) === num2term n’
-      suffices_by (
-        strip_tac
-        \\ irule replaceL2 \\ gs []
-        \\ irule_at Any sym_equation
-        \\ first_assum (irule_at Any)
-        \\ simp [proves_REFL])
-    \\ qpat_assum ‘_ = 2 * d ’ (SUBST1_TAC o SYM)
-    \\ irule num2term_BIT0 \\ gs []) *))
-  >- (
-    cheat (* bleh *))
-QED
-
-Theorem num2term_hom:
+Theorem num2term_ADD:
   numeral_thy_ok thy ⇒
     (thy,[]) |- num2term (m + n) === Comb (Comb _ADD (num2term m)) (num2term n)
 Proof
-  strip_tac
-  \\ qid_spec_tac ‘m’
+  strip_tac \\ qid_spec_tac ‘m’
   \\ gs [numeral_thy_ok_def]
   \\ Induct \\ simp []
   >- (
@@ -321,48 +196,106 @@ Proof
   \\ qmatch_goalsub_abbrev_tac ‘Comb (Comb _ADD (Comb _SUC N)) M’
   \\ ‘(thy,[]) |- Comb (Comb _ADD (Comb _SUC N)) _M ===
                   Comb _SUC (Comb (Comb _ADD N) _M)’
-    by (
-        qpat_x_assum ‘_ |- Comb (Comb _ADD _) _ === _’ assume_tac
+    by (qpat_x_assum ‘_ |- Comb (Comb _ADD _) _ === _’ assume_tac
         \\ drule_at_then (Pos (el 2)) (qspec_then ‘[N,_N]’ mp_tac) proves_INST
         \\ simp [VSUBST_def, REV_ASSOCD, equation_def, term_ok_def, Abbr ‘N’,
                  num2term_term_ok, numeral_thy_ok_def])
-  \\ ‘∀is. VSUBST is N = N’
-    by cheat (* TODO *)
   \\ ‘(thy,[]) |- Comb (Comb _ADD (Comb _SUC N)) M ===
                   Comb _SUC (Comb (Comb _ADD N) M)’
     by (drule_at_then (Pos (el 2)) (qspec_then ‘[M,_M]’ mp_tac) proves_INST
         \\ simp [VSUBST_def, REV_ASSOCD, equation_def, term_ok_def, Abbr ‘M’,
-                 num2term_term_ok, numeral_thy_ok_def])
-  \\ qspecl_then [‘t’,‘[]’,‘[]’] (irule o SIMPR []) trans_equation
-  \\ irule_at Any ACONV_REFL
+                 num2term_term_ok, numeral_thy_ok_def, Abbr ‘N’])
+  \\ irule trans_equation_simple
   \\ irule_at (Pos last) sym_equation
   \\ first_assum (irule_at Any)
-  \\ qspecl_then [‘[]’,‘[]’] (irule o SIMPR []) proves_MK_COMB
-  \\ simp [proves_REFL]
+  \\ simp [MK_COMB_simple, proves_REFL]
 QED
 
-Theorem num2bit_hom:
+Theorem ADD_num2term =
+  UNDISCH_ALL num2term_ADD |> MATCH_MP sym_equation |> DISCH_ALL;
+
+Theorem num2bit_num2term:
+  numeral_thy_ok thy ⇒
+    ∀n. (thy,[]) |- num2bit n === num2term n
+Proof
+  strip_tac \\ ho_match_mp_tac num2bit_ind \\ rw []
+  \\ gs [numeral_thy_ok_def]
+  \\ rw [num2term_def, Once num2bit_def]
+  >- (
+    qpat_assum ‘_ |- Comb _BIT0 _N === _’ assume_tac
+    \\ ‘(thy,[]) |- Comb _BIT0 _0 === Comb (Comb _ADD _0) _0’
+      by (drule_at_then (Pos (el 2)) (qspec_then ‘[_0,_N]’ mp_tac) proves_INST
+          \\ simp [VSUBST_def, REV_ASSOCD, equation_def, Once has_type_rules])
+    \\ irule trans_equation_simple
+    \\ first_x_assum (irule_at Any)
+    \\ qpat_assum ‘_ |- Comb (Comb _ADD _0) _ === _’ assume_tac
+    \\ drule_at_then (Pos (el 2)) (qspec_then ‘[_0,_M]’ mp_tac) proves_INST
+    \\ simp [VSUBST_def, REV_ASSOCD, equation_def, Once has_type_rules])
+  >- (
+    qabbrev_tac ‘N = num2term (n DIV 2)’
+    \\ ‘(thy,[]) |- Comb _BIT0 (num2bit (n DIV 2)) === Comb _BIT0 N’
+      by rw [MK_COMB_simple, proves_REFL]
+    \\ irule trans_equation_simple
+    \\ first_x_assum (irule_at Any)
+    \\ qpat_x_assum ‘_ |- Comb _BIT0 _N === _’ assume_tac
+    \\ ‘(thy,[]) |- Comb _BIT0 N === Comb (Comb _ADD N) N’
+      by (drule_at_then (Pos (el 2)) (qspec_then ‘[N,_N]’ mp_tac) proves_INST
+          \\ simp [VSUBST_def, REV_ASSOCD, equation_def, term_ok_def, Abbr ‘N’,
+                   num2term_term_ok, numeral_thy_ok_def])
+    \\ irule trans_equation_simple
+    \\ first_x_assum (irule_at Any)
+    \\ fs [Abbr ‘N’]
+    \\ qspecl_then [‘thy’,‘n DIV 2’,‘n DIV 2’] mp_tac (GEN_ALL ADD_num2term)
+    \\ gs [numeral_thy_ok_def]
+    \\ ‘2 * (n DIV 2) = n’ by intLib.ARITH_TAC \\ gs [])
+  >- (
+    qpat_assum ‘_ |- Comb _BIT1 _N === _’ assume_tac
+    \\ qabbrev_tac ‘N = num2term (n DIV 2)’
+    \\ ‘(thy,[]) |- Comb _BIT1 (num2bit (n DIV 2)) === Comb _BIT1 N’
+      by rw [MK_COMB_simple, proves_REFL]
+    \\ irule trans_equation_simple
+    \\ first_x_assum (irule_at Any)
+    \\ ‘(thy,[]) |- Comb _BIT1 N === Comb _SUC (Comb _BIT0 N)’
+      by (drule_at_then (Pos (el 2)) (qspec_then ‘[N,_N]’ mp_tac) proves_INST
+          \\ simp [VSUBST_def, REV_ASSOCD, equation_def, Once has_type_rules,
+                   num2term_term_ok, numeral_thy_ok_def, Abbr ‘N’])
+    \\ irule trans_equation_simple
+    \\ first_x_assum (irule_at Any)
+    \\ ‘n = SUC (n DIV 2 + n DIV 2)’ by intLib.ARITH_TAC
+    \\ pop_assum (fn th => simp [SimpR “(===)”, Once th])
+    \\ simp [num2term_def]
+    \\ irule MK_COMB_simple
+    \\ ‘welltyped N ∧ typeof N = num_ty’
+      by gs [Abbr ‘N’]
+    \\ simp [proves_REFL]
+    \\ ‘2 * (n DIV 2) = n DIV 2 + n DIV 2’
+      by rw []
+    \\ pop_assum SUBST1_TAC
+    \\ irule trans_equation_simple
+    \\ irule_at Any ADD_num2term
+    \\ simp [numeral_thy_ok_def]
+    \\ qpat_x_assum ‘_ |- Comb _BIT0 _N === _’ assume_tac
+    \\ drule_at_then (Pos (el 2)) (qspec_then ‘[N,_N]’ mp_tac) proves_INST
+    \\ simp [VSUBST_def, REV_ASSOCD, equation_def, term_ok_def, Abbr ‘N’,
+             num2term_term_ok, numeral_thy_ok_def, sym_equation])
+QED
+
+Theorem num2bit_ADD:
   numeral_thy_ok thy ⇒
     (thy,[]) |- num2bit (m + n) === Comb (Comb _ADD (num2bit m)) (num2bit n)
 Proof
   strip_tac
   \\ drule_then assume_tac num2bit_num2term
+  \\ first_assum (qspec_then ‘n’ assume_tac)
+  \\ first_assum (qspec_then ‘m’ assume_tac)
+  \\ first_x_assum (qspec_then ‘m + n’ assume_tac)
   \\ gs [numeral_thy_ok_def]
-  \\ ‘(thy,[]) |- Comb _ADD (num2term m) === Comb _ADD (num2bit m)’
-    by (qspecl_then [‘[]’,‘[]’] (irule o SIMPR []) proves_MK_COMB
-        \\ simp [proves_REFL, sym_equation])
-  \\ irule replaceR1
-  \\ first_x_assum (irule_at Any)
-  \\ simp [term_ok_def, num2bit_term_ok, num2term_term_ok, numeral_thy_ok_def]
-  \\ irule replaceL2 \\ simp [num2term_term_ok, numeral_thy_ok_def, term_ok_def]
-  \\ qspecl_then [‘t’,‘[]’,‘[]’] (irule_at (Pos last) o SIMPR []) trans_equation
-  \\ irule_at Any ACONV_REFL
-  \\ irule_at (Pos last) sym_equation
+  \\ irule trans_equation_simple
   \\ first_assum (irule_at Any)
-  \\ irule_at (Pos hd) sym_equation
-  \\ first_assum (irule_at Any) \\ simp [num2term_term_ok, numeral_thy_ok_def]
-  \\ irule sym_equation
-  \\ gs [numeral_thy_ok_def, num2term_hom]
+  \\ irule trans_equation_simple
+  \\ qexists_tac ‘Comb (Comb _ADD (num2term m)) (num2term n)’
+  \\ simp [num2term_ADD, numeral_thy_ok_def, MK_COMB_simple, proves_REFL,
+           sym_equation]
 QED
 
 val _ = export_theory ();
